Impl/CommitterInitModel.i.dfy
@@ -1,0 +1,99 @@
+include "CommitterModel.i.dfy"
+include "StateModel.i.dfy"
+include "IOModel.i.dfy"
+
+module CommitterInitModel {
+  import opened NativeTypes
+  import opened Options
+
+  import opened DiskLayout
+  import opened InterpretationDiskOps
+  import opened ViewOp
+  import JournalCache
+
+  import opened CommitterModel
+  import opened StateModel
+  import opened IOModel
+
+  function {:opaque} PageInSuperblockReq(k: Constants, cm: CM, io: IO, which: uint64) : (res : (CM, IO))
+  requires which == 0 || which == 1
+  requires which == 0 ==> cm.superblock1.SuperblockUnfinished?
+  requires which == 1 ==> cm.superblock2.SuperblockUnfinished?
+  requires io.IOInit?
+  requires cm.status.StatusLoadingSuperblock?
+  {
+    if which == 0 then (
+      if cm.superblock1Read.None? then (
+        var loc := Superblock1Location();
+        var (id, io') := RequestRead(io, loc);
+        var cm' := cm.(superblock1Read := Some(id));
+        (cm', io')
+      ) else (
+        (cm, io)
+      )
+    ) else (
+      if cm.superblock2Read.None? then (
+        var loc := Superblock2Location();
+        var (id, io') := RequestRead(io, loc);
+        var cm' := cm.(superblock2Read := Some(id));
+        (cm', io')
+      ) else (
+        (cm, io)
+      )
+    )
+  }
+
+  lemma PageInSuperblockReqCorrect(k: Constants,
+      cm: CM, io: IO, which: uint64)
+  requires CommitterModel.WF(cm)
+  requires PageInSuperblockReq.requires(k, cm, io, which)
+  ensures var (cm', io') := PageInSuperblockReq(k, cm, io, which);
+    && CommitterModel.WF(cm')
+    && ValidDiskOp(diskOp(io'))
+    && JournalCache.Next(Ik(k).jc,
+        CommitterModel.I(cm),
+        CommitterModel.I(cm'),
+        IDiskOp(diskOp(io')).jdop,
+        JournalInternalOp)
+  {
+    reveal_PageInSuperblockReq();
+    var (cm', io') := PageInSuperblockReq(k, cm, io, which);
+
+    var loc;
+    if which == 0 {
+      loc := Superblock1Location();
+    } else {
+      loc := Superblock2Location();
+    }
+    RequestReadCorrect(io, loc);
+
+    if (which == 0 && cm.superblock1Read.None?)
+      || (which == 1 && cm.superblock2Read.None?)
+    {
+      assert JournalCache.PageInSuperblockReq(Ik(k).jc,
+          CommitterModel.I(cm),
+          CommitterModel.I(cm'),
+          IDiskOp(diskOp(io')).jdop,
+          JournalInternalOp, which as int);
+      assert JournalCache.NextStep(Ik(k).jc,
+          CommitterModel.I(cm),
+          CommitterModel.I(cm'),
+          IDiskOp(diskOp(io')).jdop,
+          JournalInternalOp,
+          JournalCache.PageInSuperblockReqStep(which as int));
+    } else {
+      assert JournalCache.NoOp(Ik(k).jc,
+          CommitterModel.I(cm),
+          CommitterModel.I(cm'),
+          IDiskOp(diskOp(io')).jdop,
+          JournalInternalOp);
+      assert JournalCache.NextStep(Ik(k).jc,
+          CommitterModel.I(cm),
+          CommitterModel.I(cm'),
+          IDiskOp(diskOp(io')).jdop,
+          JournalInternalOp,
+          JournalCache.NoOpStep);
+
+    }
+  }
+}
